@prefix curric: <https://w3id.org/uk/curriculum/core/> .
@prefix eng: <https://w3id.org/uk/curriculum/england/> .
@prefix rdf: <http://www.w3.org/1999/02/22-rdf-syntax-ns#> .
@prefix rdfs: <http://www.w3.org/2000/01/rdf-schema#> .
@prefix owl: <http://www.w3.org/2002/07/owl#> .
@prefix skos: <http://www.w3.org/2004/02/skos/core#> .
@prefix dc: <http://purl.org/dc/elements/1.1/> .
@prefix dcterms: <http://purl.org/dc/terms/> .
@prefix vann: <http://purl.org/vocab/vann/> .
@prefix xsd: <http://www.w3.org/2001/XMLSchema#> .

# ======================================================================
# National Curriculum for England - History Knowledge Taxonomy 
# ======================================================================

# ----------------------------------------------------------------------
# Ontology Declaration
# ----------------------------------------------------------------------

<https://w3id.org/uk/curriculum/england/history-knowledge-taxonomy>
  rdf:type owl:Ontology ;

  rdfs:label "National Curriculum for England - History Knowledge Taxonomy"@en ;
  dc:title "National Curriculum for England - History Knowledge Taxonomy"@en ;
  rdfs:comment """History knowledge taxonomy defining the hierarchical organization of historical 
  content from strands through to content sub-descriptors."""@en ;

  owl:versionInfo "0.1.0" ;
  owl:versionIRI <https://w3id.org/uk/curriculum/england/history-knowledge-taxonomy/0.1.0> ;
  owl:priorVersion <https://w3id.org/uk/curriculum/england/history-knowledge-taxonomy/0.0.9> ;
  
  dcterms:description """This file defines the History knowledge taxonomy for the National 
  Curriculum in England, organizing content through strands, sub-strands, content descriptors, 
  and content sub-descriptors."""@en ;
  dc:creator "Department for Education" ;
  dcterms:created "2025-11-24"^^xsd:date ;
  dcterms:modified "2025-12-03"^^xsd:date ;
  dcterms:issued "2025-12-03"^^xsd:date ;
  
  dcterms:license <http://www.nationalarchives.gov.uk/doc/open-government-licence/version/3/> ;
  dcterms:rights "Crown Copyright"@en ;

  rdfs:seeAlso <https://www.gov.uk/government/collections/national-curriculum> ;
  vann:preferredNamespacePrefix "eng" ;
  vann:preferredNamespaceUri "https://w3id.org/uk/curriculum/england/" ;

  owl:imports <https://w3id.org/uk/curriculum/core/> ;
  owl:imports <https://w3id.org/uk/curriculum/england/history-subject> .

# ----------------------------------------------------------------------
# Knowledge Taxonomy
# ----------------------------------------------------------------------

eng:knowledge-taxonomy
  a skos:ConceptScheme ;
  skos:prefLabel "National Curriculum for England Knowledge Structure"@en ;
  skos:hasTopConcept eng:discipline-history .
  
# ----------------------------------------------------------------------
# Disciplines
# ----------------------------------------------------------------------

eng:discipline-history
  a skos:Concept, curric:Discipline ;
  skos:prefLabel "History"@en ;
  skos:topConceptOf eng:knowledge-taxonomy ;
  skos:definition """The national curriculum for history develops knowledge and understanding of 
  Britain’s past and that of the wider world."""@en ;
  skos:scopeNote """History helps pupils to understand the complexity of people’s lives, the 
  process of change, the diversity of societies and relationships between different groups, as well 
  as their own identity and the challenges of their time. It equips pupils to ask perceptive 
  questions, think critically, weigh evidence, sift arguments, and develop perspective and 
  judgement."""@en ;
  skos:narrower eng:strand-knowledge-of-past ,
                eng:strand-knowledge-of-history ;
  skos:inScheme eng:knowledge-taxonomy .

# ----------------------------------------------------------------------
# Strands
# ----------------------------------------------------------------------

eng:strand-knowledge-of-past
  a skos:Concept, curric:Strand ;
  skos:prefLabel "Knowledge of the past"@en ;
  skos:broader eng:discipline-history ;
  skos:narrower eng:substrand-cells-organisation ,
                eng:substrand-skeletal-and-muscular-systems ;
  skos:inScheme eng:knowledge-taxonomy .

eng:strand-knowledge-of-history
  a skos:Concept, curric:Strand ;
  skos:prefLabel "Knowledge of history as a discipline"@en ;
  skos:broader eng:discipline-history ;
  skos:narrower eng:substrand-cells-organisation ,
                eng:substrand-skeletal-and-muscular-systems ;
  skos:inScheme eng:knowledge-taxonomy .

# ----------------------------------------------------------------------
# Sub-Strands
# ----------------------------------------------------------------------

eng:substrand-cells-organisation
  a skos:Concept, curric:SubStrand ;
  skos:prefLabel "Cells and organisation"@en ;
  skos:broader eng:strand-structure-function-living-organisms ;
  skos:narrower eng:content-descriptor-cells-as-unit-of-living-organism ,
                eng:content-descriptor-functions-of-the-cell-wall ;
  skos:inScheme eng:knowledge-taxonomy .



# ----------------------------------------------------------------------
# Content Descriptors
# ----------------------------------------------------------------------

eng:content-descriptor-cells-as-unit-of-living-organism
  a skos:Concept, curric:ContentDescriptor ;
  skos:prefLabel """Cells as the fundamental unit of living organisms, including how to observe, 
  interpret and record cell structure using a light microscope."""@en ;
  skos:broader eng:substrand-cells-organisation ;
  skos:inScheme eng:knowledge-taxonomy .



# ----------------------------------------------------------------------
# Content Sub-Descriptors
# ----------------------------------------------------------------------

eng:content-subdescriptor-seasons-detail
  a skos:Concept, curric:ContentSubDescriptor ;
  skos:prefLabel "Seasons detail"@en ;
  skos:broader eng:content-descriptor-observe-seasonal-changes ;
  skos:inScheme eng:knowledge-taxonomy .
